Superposition_Calculus/Functional_Substitution.thy
@@ -28,6 +28,18 @@ locale renaming_variables =
     renaming_variables:
       "\<And>expr \<rho>. is_renaming \<rho> \<Longrightarrow> id_subst ` vars (subst expr \<rho>) = \<rho> ` (vars expr)"
 
+locale variables_in_base_imgu =
+  fixes 
+    base_is_imgu and
+    vars :: "'expr \<Rightarrow> 'var set" and
+    subst:: "'expr \<Rightarrow> ('var \<Rightarrow> 'base) \<Rightarrow> 'expr" and
+    base_vars :: "'base \<Rightarrow> 'var set"
+  assumes
+    variables_in_base_imgu: "\<And>expr \<mu> unifications.
+      base_is_imgu \<mu> unifications \<Longrightarrow>
+      finite unifications \<Longrightarrow> \<forall>unification \<in> unifications. finite unification \<Longrightarrow>
+      vars (subst expr \<mu>) \<subseteq> vars expr \<union> (\<Union>(base_vars ` \<Union> unifications))"
+
 locale functional_substitution = substitution _ _ subst "\<lambda>a. vars a = {}" 
   for
     subst :: "'expr \<Rightarrow> ('var \<Rightarrow> 'base) \<Rightarrow> 'expr" (infixl "\<cdot>" 70) and
@@ -234,55 +246,5 @@ lemma variable_grounding:
   by blast
 
 end
-
-locale variables_in_base_imgu =
-  fixes 
-    base_is_imgu and
-    vars :: "'expr \<Rightarrow> 'var set" and
-    subst:: "'expr \<Rightarrow> ('var \<Rightarrow> 'base) \<Rightarrow> 'expr" and
-    base_vars :: "'base \<Rightarrow> 'var set"
-  assumes
-    variables_in_base_imgu: "\<And>expr \<mu> unifications. 
-      base_is_imgu \<mu> unifications \<Longrightarrow> 
-      finite unifications \<Longrightarrow> \<forall>unification \<in> unifications. finite unification \<Longrightarrow>  
-      vars (subst expr \<mu>) \<subseteq> vars expr \<union> (\<Union>(base_vars ` \<Union> unifications))"
-
-locale base_variables_in_base_imgu = base_functional_substitution +
-  assumes
-    variables_in_base_imgu: "\<And>expr \<mu> unifications. 
-      is_imgu \<mu> unifications \<Longrightarrow> 
-      finite unifications \<Longrightarrow> \<forall>unification \<in> unifications. finite unification \<Longrightarrow>  
-      vars (subst expr \<mu>) \<subseteq> vars expr \<union> (\<Union>(vars ` \<Union> unifications))"
-begin
-
-
-end
-
-
-(*locale based_variables_in_base_imgu = 
-  based_functional_substitution + 
-  base: base_variables_in_base_imgu where subst = base_subst and vars = base_vars
-begin
-
-sublocale variables_in_base_imgu where base_is_imgu = base.is_imgu
-proof unfold_locales
-  fix expr \<mu> unifications
-  assume imgu_vars:
-    "base.is_imgu \<mu> unifications" 
-    "finite unifications" 
-    "\<forall>unification\<in>unifications. finite unification"
-
-  show "vars (expr \<cdot> \<mu>) \<subseteq> vars expr \<union> \<Union> (base_vars ` \<Union> unifications)"
-    using base.variables_in_base_imgu[OF imgu_vars]
-    
-    sorry
-qed
-
-end*)
-  (*assumes
-    variables_in_base_imgu: "\<And>expr \<mu> unifications. 
-      base.is_imgu \<mu> unifications \<Longrightarrow> 
-      finite unifications \<Longrightarrow> \<forall>unification \<in> unifications. finite unification \<Longrightarrow>  
-      vars (subst expr \<mu>) \<subseteq> vars expr \<union> (\<Union>(base_vars ` \<Union> unifications))"*)
 
 end
