Superposition_Calculus/Functional_Substitution_Lifting.thy
@@ -2,22 +2,38 @@ theory Functional_Substitution_Lifting
   imports Functional_Substitution
 begin
 
+locale natural_functor =
+  fixes
+    map :: "('a \<Rightarrow> 'a) \<Rightarrow> 'b \<Rightarrow> 'b" and
+    to_set :: "'b \<Rightarrow> 'a set"
+  assumes
+    map_comp: "\<And>b f g. map (f \<circ> g) b = map f (map g b)" and
+    map_id: "\<And>b. map id b = b" and
+    map_cong: "\<And>b f g. (\<And>a. a \<in> to_set b \<Longrightarrow> f a = g a) \<Longrightarrow> map f b = map g b" and
+    to_set_map: "\<And>b f. to_set (map f b) = f ` to_set b" and
+    exists_functor: "\<And>a. \<exists>b. a \<in> to_set b"
+
+locale natural_functor_conversion =
+  natural_functor +
+  fixes
+    map_to :: "('a \<Rightarrow> 'b) \<Rightarrow> 'c \<Rightarrow> 'd" and
+    map_from :: "('b \<Rightarrow> 'a) \<Rightarrow> 'd \<Rightarrow> 'c" and
+    map' :: "('b \<Rightarrow> 'b) \<Rightarrow> 'd \<Rightarrow> 'd" and
+    to_set' :: "'d \<Rightarrow> 'b set"
+  assumes
+    to_set_map_from: "\<And>f d. to_set (map_from f d) = f ` to_set' d" and
+    conversion_map_comp: "\<And>c f g. map (f \<circ> g) c = map_from f (map_to g c)" and
+    map'_comp: "\<And>d f g. map' (f \<circ> g) d = map_to f (map_from g d)" and
+    map'_id: "\<And>d. map' id d = d"
+
 locale functional_substitution_lifting = 
-  sub: functional_substitution
-  where subst = sub_subst and vars = sub_vars
+  sub: functional_substitution where subst = sub_subst and vars = sub_vars +
+  natural_functor where map = map and to_set = to_set
   for
     sub_vars :: "'sub \<Rightarrow> 'var set" and
-    sub_subst :: "'sub \<Rightarrow> ('var \<Rightarrow> 'base) \<Rightarrow> 'sub" +
-  fixes
+    sub_subst :: "'sub \<Rightarrow> ('var \<Rightarrow> 'base) \<Rightarrow> 'sub" and
     map :: "('sub \<Rightarrow> 'sub) \<Rightarrow> 'expr \<Rightarrow> 'expr" and
     to_set :: "'expr \<Rightarrow> 'sub set"
-  assumes
-    map_comp: "\<And>expr f g. map (f \<circ> g) expr = map f (map g expr)" and
-    map_id: "map id expr = expr" and
-    map_cong: 
-      "\<And>expr f g. (\<And>sub. sub \<in> to_set expr \<Longrightarrow> f sub = g sub) \<Longrightarrow> map f expr = map g expr" and
-    to_set_map: "\<And>expr f. to_set (map f expr) = f ` to_set expr" and
-    exists_expression: "\<And>sub. \<exists>expr. sub \<in> to_set expr" 
 begin
 
 definition vars :: "'expr \<Rightarrow> 'var set" where
@@ -86,7 +102,7 @@ proof(unfold is_ground_subst_def sub.is_ground_subst_def, intro iffI allI)
     assume sub_not_ground: "\<not>sub.is_ground (sub \<cdot>\<^sub>s \<gamma>)"
 
     then obtain expr where "sub \<in> to_set expr"
-      using exists_expression by auto
+      using exists_functor by blast
 
     then have "\<not>is_ground (expr \<cdot> \<gamma>)"
       using sub_not_ground to_set_map 
@@ -137,10 +153,8 @@ lemma to_set_image: "to_set (expr \<cdot> \<sigma>) = (\<lambda>a. a \<cdot>\<^s
 end
 
 locale based_functional_substitution_lifting = 
-  base: base_functional_substitution 
-  where subst = base_subst and vars = base_vars +
-  functional_substitution_lifting
-  where to_set = to_set
+  base: base_functional_substitution where subst = base_subst and vars = base_vars +
+  functional_substitution_lifting where to_set = to_set
   for base_subst :: "'base \<Rightarrow> ('var \<Rightarrow> 'base) \<Rightarrow> 'base" and base_vars 
     and to_set :: "'expr \<Rightarrow> 'sub set" +
   assumes 
@@ -190,8 +204,8 @@ end
 
 locale renaming_variables_lifting = 
   functional_substitution_lifting +
-  sub: renaming_variables 
-  where vars = sub_vars and subst = sub_subst and is_renaming = sub.is_renaming
+  sub: renaming_variables where vars = sub_vars and subst = sub_subst and 
+  is_renaming = sub.is_renaming
 begin
 
 sublocale renaming_variables where subst = subst and vars = vars and is_renaming = is_renaming
@@ -209,12 +223,11 @@ end
 
 locale variables_in_base_imgu_lifting = 
   based_functional_substitution_lifting +
-  sub: variables_in_base_imgu 
-    where vars = sub_vars and subst = sub_subst and base_is_imgu = base.is_imgu
+  sub: variables_in_base_imgu where vars = sub_vars and subst = sub_subst and 
+  base_is_imgu = base.is_imgu
 begin
 
-sublocale variables_in_base_imgu where 
-  subst = subst and vars = vars and base_is_imgu = base.is_imgu
+sublocale variables_in_base_imgu where subst = subst and vars = vars and base_is_imgu = base.is_imgu
 proof unfold_locales
   fix expr \<mu> unifications
   assume imgu: 
@@ -231,29 +244,22 @@ qed
 end
 
 locale grounding_lifting = 
-  functional_substitution_lifting 
-  where sub_vars = sub_vars and sub_subst = sub_subst and map = map + 
-  sub: grounding
-  where vars = sub_vars and subst = sub_subst and to_ground = sub_to_ground and 
-    from_ground = sub_from_ground 
+  functional_substitution_lifting where sub_vars = sub_vars and sub_subst = sub_subst and 
+  map = map + 
+  sub: grounding where vars = sub_vars and subst = sub_subst and to_ground = sub_to_ground and 
+  from_ground = sub_from_ground +
+  natural_functor_conversion where map = map and map_to = to_ground_map and 
+  map_from = from_ground_map and map' = ground_map and to_set' = to_set_ground
   for
     sub_to_ground :: "'sub \<Rightarrow> 'sub\<^sub>G" and 
     sub_from_ground :: "'sub\<^sub>G \<Rightarrow> 'sub" and
     sub_vars :: "'sub \<Rightarrow> 'var set" and 
     sub_subst :: "'sub \<Rightarrow> ('var \<Rightarrow> 'base) \<Rightarrow> 'sub" and
-    map :: "('sub \<Rightarrow> 'sub) \<Rightarrow> 'expr \<Rightarrow> 'expr" +
-  fixes
+    map :: "('sub \<Rightarrow> 'sub) \<Rightarrow> 'expr \<Rightarrow> 'expr" and
     to_ground_map :: "('sub \<Rightarrow> 'sub\<^sub>G) \<Rightarrow> 'expr \<Rightarrow> 'expr\<^sub>G" and
     from_ground_map :: "('sub\<^sub>G \<Rightarrow> 'sub) \<Rightarrow> 'expr\<^sub>G \<Rightarrow> 'expr" and
     ground_map :: "('sub\<^sub>G \<Rightarrow> 'sub\<^sub>G) \<Rightarrow> 'expr\<^sub>G \<Rightarrow> 'expr\<^sub>G" and
     to_set_ground :: "'expr\<^sub>G \<Rightarrow> 'sub\<^sub>G set"
-  assumes 
-    to_set_from_ground_map: 
-      "\<And>expr\<^sub>G f. to_set (from_ground_map f expr\<^sub>G) = f ` to_set_ground expr\<^sub>G" and
-    map_ground_comp: "\<And>expr f g. map (f \<circ> g) expr = from_ground_map f (to_ground_map g expr)" and
-    ground_map_comp: 
-      "\<And>expr\<^sub>G f g. ground_map (f \<circ> g) expr\<^sub>G = to_ground_map f (from_ground_map g expr\<^sub>G)" and
-    ground_map_id: "\<And>expr\<^sub>G. ground_map id expr\<^sub>G = expr\<^sub>G"
 begin
 
 definition to_ground :: "'expr \<Rightarrow> 'expr\<^sub>G" where 
@@ -278,7 +284,7 @@ proof unfold_locales
       by fast
 
     then have "\<exists>expr\<^sub>G. from_ground expr\<^sub>G = expr"
-      using map_ground_comp[symmetric] map_id_cong
+      using conversion_map_comp[symmetric] map_id_cong
       unfolding from_ground_def comp_def
       by metis
 
@@ -295,21 +301,21 @@ proof unfold_locales
 
     then show False
       unfolding vars_def from_ground_def
-      using sub.ground_is_ground to_set_from_ground_map by auto
+      using sub.ground_is_ground to_set_map_from by auto
   qed
 
   ultimately show "{expr. is_ground expr} = range from_ground"
     by blast   
 next
   show "\<And>expr\<^sub>G. to_ground (from_ground expr\<^sub>G) = expr\<^sub>G"
-    using ground_map_id
+    using map'_id
     unfolding from_ground_def to_ground_def 
-    by (metis ground_map_comp sub.to_ground_from_ground_id)
+    by (metis map'_comp sub.to_ground_from_ground_id)
 qed
 
 lemma to_set_from_ground: "to_set (from_ground expr) = sub_from_ground ` (to_set_ground expr)"
   unfolding from_ground_def
-  by (simp add: to_set_from_ground_map)
+  by (simp add: to_set_map_from)
 
 lemma sub_in_ground_is_ground: 
   assumes "sub \<in> to_set (from_ground expr)" 
@@ -329,11 +335,10 @@ lemma ground_sub:
 end
 
 locale all_subst_ident_iff_ground_lifting = 
-  finite_variables_lifting 
-  where map = map and id_subst = id_subst +  
-  sub: all_subst_ident_iff_ground 
-  where subst = sub_subst and is_ground = sub.is_ground
-  for map :: "('sub \<Rightarrow> 'sub) \<Rightarrow> 'expr \<Rightarrow> 'expr" and id_subst :: "'var \<Rightarrow> 'base"
+  finite_variables_lifting where map = map and id_subst = id_subst +  
+  sub: all_subst_ident_iff_ground where subst = sub_subst and is_ground = sub.is_ground
+for 
+  map :: "('sub \<Rightarrow> 'sub) \<Rightarrow> 'expr \<Rightarrow> 'expr" and id_subst :: "'var \<Rightarrow> 'base"
 begin
 
 sublocale all_subst_ident_iff_ground where subst = subst and is_ground = is_ground
