Superposition_Calculus/Nonground_Context.thy
@@ -6,331 +6,116 @@ begin
 
 section \<open>Nonground Contexts and Substitutions\<close>
 
-find_consts "('f,'a) actxt \<Rightarrow> 'a set"
+lemma finite_set2_actxt: "finite (set2_actxt c)"
+  by(induction c) auto
 
-lemma xx: "finite (set2_actxt c)"
-  apply(induction c)
-  by auto
+global_interpretation "context": natural_functor where map = map_args_actxt and to_set = set2_actxt
+proof unfold_locales
+  show "\<And>t. \<exists>c. t \<in> set2_actxt c"
+    by (metis actxt.set_intros(5) list.set_intros(1))
+qed (auto 
+    simp: actxt.set_map(2) actxt.map_comp fun.map_ident actxt.map_ident_strong 
+    cong: actxt.map_cong)
 
-locale clause_lifting' =
-  based_functional_substitution_lifting where 
-  base_subst = "(\<cdot>t)" and base_vars = term.vars and id_subst = Var and comp_subst = "(\<odot>)" + 
-  all_subst_ident_iff_ground_lifting where id_subst = Var and comp_subst = "(\<odot>)" +
-  grounding_lifting where id_subst = Var and comp_subst = "(\<odot>)" +
-  renaming_variables_lifting where id_subst = Var and comp_subst = "(\<odot>)" +
-  variables_in_base_imgu_lifting where id_subst = Var and comp_subst = "(\<odot>)" and base_subst = "(\<cdot>t)" and base_vars = term.vars 
+global_interpretation "context": natural_functor_conversion 
+  where map = map_args_actxt and to_set = set2_actxt and map_to = map_args_actxt 
+    and map_from = map_args_actxt and map' = map_args_actxt and to_set' = set2_actxt
+  by unfold_locales
+    (auto simp: actxt.set_map(2) actxt.map_comp cong: actxt.map_cong)
 
-global_interpretation "context": clause_lifting' where 
-    sub_vars = term.vars and sub_subst = "(\<cdot>t)" and to_set = "set2_actxt" and map = "map_args_actxt"
+global_interpretation "context": lifting_from_term where 
+    sub_vars = term.vars and sub_subst = "(\<cdot>t)" and to_set = "set2_actxt" and map = map_args_actxt
     and sub_to_ground = term.to_ground and sub_from_ground = term.from_ground 
-    and to_ground_map = map_args_actxt and from_ground_map = map_args_actxt and ground_map = map_args_actxt
-    and to_set_ground = set2_actxt
+    and to_ground_map = map_args_actxt and from_ground_map = map_args_actxt 
+    and ground_map = map_args_actxt and to_set_ground = set2_actxt
    rewrites 
     "\<And>c. context.vars c = vars_ctxt c" and 
     "\<And>c \<sigma>. context.subst c \<sigma> = c \<cdot>\<^sub>c \<sigma>"
-    apply unfold_locales
-          apply (simp add: actxt.map_comp fun.map_ident)
-         apply (simp add: actxt.map_cong)
-        apply (metis actxt.map_cong)
-       apply (simp add: actxt.set_map(2))
-            apply (metis actxt.set_intros(5) in_set_conv_decomp)
-           apply (meson is_ground_iff)
+proof -
+  interpret lifting_from_term term.vars "(\<cdot>t)" map_args_actxt set2_actxt term.to_ground
+    term.from_ground map_args_actxt map_args_actxt map_args_actxt set2_actxt
+    by unfold_locales (auto simp: is_ground_iff finite_set2_actxt)
 
-          apply (simp add: actxt.set_map(2))
-  apply (simp add: xx)
-        apply (simp add: actxt.map_comp fun.map_ident)
-  apply (simp add: actxt.set_map(2))
-       apply (simp add: actxt.map_comp fun.map_ident)
-  apply (simp add: actxt.map_comp fun.map_ident)
-    apply (simp add: actxt.map_cong)
-  (* TODO *)
-  sorry
-
-
-(*global_interpretation "context":
-  grounding_lifting where 
-    id_subst = Var and comp_subst = "(\<odot>)" and 
-    sub_vars = term.vars and sub_subst = "(\<cdot>t)" and to_set = "set2_actxt" and map = "map_args_actxt"
-    and sub_to_ground = term.to_ground and sub_from_ground = term.from_ground 
-    and to_ground_map = map_args_actxt and from_ground_map = map_args_actxt and ground_map = map_args_actxt
-    and to_set_ground = set2_actxt
-  rewrites 
-    "\<And>c. context.vars c = vars_ctxt c" and 
-    "\<And>c \<sigma>. context.subst c \<sigma> = c \<cdot>\<^sub>c \<sigma>"
-  apply unfold_locales
-          apply (simp add: actxt.map_comp fun.map_ident)
-         apply (simp add: actxt.map_cong)
-        apply (metis actxt.map_cong)
-       apply (simp add: actxt.set_map(2))
-      apply (metis actxt.set_intros(5) in_set_conv_decomp)
-     apply (simp add: actxt.set_map(2))
-    apply (simp add: actxt.map_comp fun.map_ident)
-   apply (simp add: actxt.map_comp fun.map_ident)
-    apply (simp add: actxt.map_cong)
-  sorry
-
-global_interpretation "context": based_functional_substitution_lifting 
-  where comp_subst = "(\<odot>)"  and id_subst = Var and sub_vars = term.vars and sub_subst = "(\<cdot>t)"
-    and to_set = "set2_actxt" and map = "map_args_actxt" and base_subst = "(\<cdot>t)" 
-    and base_vars = term.vars
-  (*rewrites 
-    "\<And>c. context.vars c = vars_ctxt c" and 
-    "\<And>c \<sigma>. context.subst c \<sigma> = c \<cdot>\<^sub>c \<sigma>"*) +
-  all_subst_ident_iff_ground_lifting where 
-    id_subst = Var and comp_subst = "(\<odot>)"  and sub_vars = term.vars and sub_subst = "(\<cdot>t)" and to_set = "set2_actxt" and map = "map_args_actxt"
-proof-
-  interpret based_functional_substitution_lifting 
-    where comp_subst = "(\<odot>)"  and id_subst = Var and sub_vars = term.vars and sub_subst = "(\<cdot>t)"
-      and to_set = "set2_actxt" and map = "map_args_actxt" and base_subst = "(\<cdot>t)" 
-      and base_vars = term.vars
-  proof unfold_locales
-    show "\<And>expr \<gamma>. (term.vars (expr \<cdot>t \<gamma>) = {}) = (\<forall>var\<in>term.vars expr. term.vars (\<gamma> var) = {})"
-      by (simp add: is_ground_iff)
-  qed auto
-
- fix c :: "('a, ('f, 'v) Term.term) actxt"
-  show "context.vars c = vars_ctxt c"
-    unfolding context.vars_def 
-    apply(induction c) 
-    by auto
+  fix c :: "('a, ('f, 'v) Term.term) actxt"
+  show "vars c = vars_ctxt c"
+    unfolding vars_def 
+    by(induction c) auto
 
   fix \<sigma> 
-  show "context.subst c \<sigma> = c \<cdot>\<^sub>c \<sigma>"
-  by blast
+  show "subst c \<sigma> = c \<cdot>\<^sub>c \<sigma>"
+    unfolding subst_def
+    by blast
 
-  show "based_functional_substitution_lifting (\<odot>) Var term.vars (\<cdot>t) map_args_actxt (\<cdot>t) term.vars set2_actxt"
+  show "lifting_from_term term.vars (\<cdot>t) map_args_actxt set2_actxt term.to_ground term.from_ground
+     map_args_actxt map_args_actxt map_args_actxt set2_actxt"
     by unfold_locales
-
-  show "all_subst_ident_iff_ground_lifting (\<odot>) term.vars (\<cdot>t) set2_actxt map_args_actxt Var"
-  proof unfold_locales
-    fix c :: "('l, ('k, 'j) Term.term) actxt"
-    show "finite (set2_actxt c)"
-      apply(induction c)
-      by auto
-  qed
 qed
-
-global_interpretation "context": all_subst_ident_iff_ground_lifting where 
-  id_subst = Var and comp_subst = "(\<odot>)" and sub_vars = term.vars and sub_subst = "(\<cdot>t)"
-  and to_set = "set2_actxt" and map = "map_args_actxt"
-proof unfold_locales
-  fix c :: "('c, ('b, 'a) Term.term) actxt"
-  show "finite (set2_actxt c)"
-    apply(induction c)
-    by auto
-qed*)
-
-(* TODO: Try how much can be generalized using abstract contexts 
-global_interpretation "context": all_subst_ident_iff_ground where 
-  is_ground = "\<lambda>c. context.vars c = {}" and subst = "(\<cdot>t\<^sub>c)"
-proof unfold_locales
-  fix c :: "('f, 'v) context"
-  show "context.vars c = {} = (\<forall>\<sigma>. c \<cdot>t\<^sub>c \<sigma> = c)"
-  proof (intro iffI)
-    show "context.vars c = {} \<Longrightarrow> \<forall>\<sigma>. c \<cdot>t\<^sub>c \<sigma> = c"
-      by(induction c) (simp_all add: list.map_ident_strong)
-  next
-    assume "\<forall>\<sigma>. c \<cdot>t\<^sub>c \<sigma> = c"
-
-    then have "\<And>t\<^sub>G. term.is_ground t\<^sub>G \<Longrightarrow> \<forall>\<sigma>. c\<langle>t\<^sub>G\<rangle> \<cdot>t \<sigma> = c\<langle>t\<^sub>G\<rangle>"
-      by simp
-
-    then have "\<And>t\<^sub>G. term.is_ground t\<^sub>G \<Longrightarrow> term.is_ground c\<langle>t\<^sub>G\<rangle>"
-      by (meson is_ground_trm_iff_ident_forall_subst)
-
-    then show "context.vars c = {}"
-      by (metis sup.commute sup_bot_left vars_term_ctxt_apply vars_term_of_gterm)
-  qed
-next
-  fix c :: "('f, 'v) context" and cs :: "('f, 'v) context set"
-  assume finite: "finite cs" and non_ground: "context.vars c \<noteq> {}"
-
-  then show "\<exists>\<sigma>. c \<cdot>t\<^sub>c \<sigma> \<noteq> c \<and> c \<cdot>t\<^sub>c \<sigma> \<notin> cs"
-  proof(induction c arbitrary: cs)
-    case Hole
-    then show ?case
-      by simp
-  next
-    case (More f ts c ts')
-
-    show ?case
-    proof(cases "context.vars c = {}")
-      case True
-
-      let ?sub_terms = 
-        "\<lambda>c :: ('f, 'v) context. case c of More _ ts _ ts' \<Rightarrow> set ts \<union> set ts'  | _ \<Rightarrow> {}"
-
-      let ?cs' = "set ts \<union> set ts' \<union> \<Union>(?sub_terms ` cs)"
-
-      from True obtain t where t: "t \<in> set ts \<union> set ts'" and non_ground: "\<not>term.is_ground t"
-        using More.prems by auto
-
-      have "\<And>c. finite (?sub_terms c)"
-      proof-  
-        fix c
-        show "finite (?sub_terms c)"
-          by(cases c) simp_all
-      qed
-
-      then have "finite (\<Union>(?sub_terms ` cs))"
-        using More.prems(1) by blast
-
-      then have finite: "finite ?cs'"
-        by blast
-
-      obtain \<sigma> where \<sigma>: "t \<cdot>t \<sigma> \<noteq> t" and cs': "t \<cdot>t \<sigma> \<notin> ?cs'"
-        using term.exists_non_ident_subst[OF finite non_ground]
-        by blast
-
-      then have "More f ts c ts' \<cdot>t\<^sub>c \<sigma> \<noteq> More f ts c ts'"
-        using t set_map_id[of _  _ "\<lambda>t. t \<cdot>t \<sigma>"]
-        by auto
-
-      moreover have " More f ts c ts' \<cdot>t\<^sub>c \<sigma> \<notin> cs"
-        using cs' t
-        by auto
-
-      ultimately show ?thesis
-        by blast
-    next
-      case False
-
-      let ?sub_contexts = "(\<lambda>c. case c of More _ _ c _ \<Rightarrow> c) ` {c \<in> cs. c \<noteq> \<box>}"
-
-      have "finite ?sub_contexts"
-        using More.prems(1)
-        by auto
-
-      then obtain \<sigma> where \<sigma>: "c \<cdot>t\<^sub>c \<sigma> \<noteq> c" and sub_contexts: "c \<cdot>t\<^sub>c \<sigma> \<notin> ?sub_contexts"
-        using More.IH[OF _ False]
-        by blast
-
-      then have "More f ts c ts' \<cdot>t\<^sub>c \<sigma> \<noteq> More f ts c ts'"
-        by simp
-
-      moreover have "More f ts c ts' \<cdot>t\<^sub>c \<sigma> \<notin> cs"
-        using sub_contexts image_iff
-        by fastforce
-
-      ultimately show ?thesis 
-        by blast
-    qed
-  qed
-qed
-*)
-(*global_interpretation "context": based_functional_substitution where
-  subst = "(\<cdot>t\<^sub>c)" and vars = context.vars and id_subst = Var and comp_subst = "(\<odot>)" and 
-  base_vars = term.vars and base_subst = "(\<cdot>t)"
-proof(unfold_locales, unfold substitution_ops.is_ground_subst_def)
-  fix c :: "('f, 'v) context"
-  show "c \<cdot>t\<^sub>c Var = c"
-    by (induction c) auto
-next
-  show "\<And>c \<sigma> \<tau>. c \<cdot>t\<^sub>c \<sigma> \<odot> \<tau> = c \<cdot>t\<^sub>c \<sigma> \<cdot>t\<^sub>c \<tau>"
-    by simp
-next
-  show "\<And>c. context.vars c = {} \<Longrightarrow> \<forall>\<sigma>. c \<cdot>t\<^sub>c \<sigma> = c"
-    using context.all_subst_ident_iff_ground by blast
-next 
-  show "\<And>c \<sigma> \<tau>. (\<And>x. x \<in> context.vars c \<Longrightarrow> \<sigma> x = \<tau> x) \<Longrightarrow> c \<cdot>t\<^sub>c \<sigma> = c \<cdot>t\<^sub>c \<tau>"
-    using ctxt_subst_eq.
-next
-  fix \<gamma> :: "('f,'v) subst"
-
-  show "(\<forall>c. context.vars (c \<cdot>t\<^sub>c \<gamma>) = {}) \<longleftrightarrow> (\<forall>t. term.vars (t \<cdot>t \<gamma>) = {})"
-  proof(intro iffI allI equals0I)
-    fix t x
-
-    assume is_ground: "\<forall>c. context.vars (c \<cdot>t\<^sub>c \<gamma>) = {}" and vars: "x \<in> term.vars (t \<cdot>t \<gamma>)"
-
-    have "\<And>f. context.vars (More f [t] Hole [] \<cdot>t\<^sub>c \<gamma>) = {}"
-      using is_ground
-      by presburger
-
-    moreover have "\<And>f. x \<in> context.vars (More f [t] Hole [] \<cdot>t\<^sub>c \<gamma>)"
-      using vars
-      by simp
-
-    ultimately show False
-      by blast
-  next
-    fix c x
-    assume is_ground: "\<forall>t. term.is_ground (t \<cdot>t \<gamma>)" and vars: "x \<in> context.vars (c \<cdot>t\<^sub>c \<gamma>)"
-
-    have "\<And>t. term.is_ground (c\<langle>t\<rangle> \<cdot>t \<gamma>)"
-      using is_ground
-      by presburger
-
-    moreover have "\<And>t. x \<in> term.vars (c\<langle>t\<rangle> \<cdot>t \<gamma>)"
-      using vars
-      by simp
-
-    ultimately show False
-      by blast
-  qed
-next
-  fix c and \<gamma> :: "('f, 'v) subst"
-
-  show "context.vars (c \<cdot>t\<^sub>c \<gamma>) = {} \<longleftrightarrow> (\<forall>x \<in> context.vars c. term.is_ground (\<gamma> x))"
-    by(induction c)(auto simp: term.is_grounding_iff_vars_grounded)
-qed
-
-global_interpretation "context": finite_variables 
-  where vars = "context.vars :: ('f, 'v) context \<Rightarrow> 'v set"
-proof unfold_locales
-  fix c :: "('f, 'v) context"
-
-  have "\<And>t. finite (term.vars c\<langle>t\<rangle>)"
-    using term.finite_vars by blast
-
-  then show "finite (context.vars c)"
-    unfolding vars_term_ctxt_apply finite_Un
-    by simp
-qed*)
-
-(*global_interpretation "context": grounding where 
-  vars = "context.vars :: ('f, 'v) context \<Rightarrow> 'v set" and id_subst = Var and comp_subst = "(\<odot>)" and 
-  subst = "(\<cdot>t\<^sub>c)" and from_ground = context.from_ground and to_ground = context.to_ground
-proof unfold_locales
-  have "\<And>c. context.vars c = {} \<Longrightarrow> \<exists>c\<^sub>G. context.from_ground c\<^sub>G = c"
-    by (metis Un_empty_left gctxt_of_ctxt_inv term.ground_exists term.to_ground_inverse 
-        term_of_gterm_ctxt_apply_ground(1) vars_term_ctxt_apply)
-
-  then show "{c. context.vars c = {}} = range context.from_ground"
-    by force
-next 
-  show "\<And>c\<^sub>G. context.to_ground (context.from_ground c\<^sub>G) = c\<^sub>G"
-    by simp
-qed
-
-global_interpretation  
-  "context": renaming_variables where vars = context.vars and 
-  is_renaming = context.is_renaming and id_subst = Var and subst = "(\<cdot>t\<^sub>c)" +
-  "context": variables_imgu where vars = context.vars and base_is_imgu = term_subst.is_imgu and 
-  subst = "(\<cdot>t\<^sub>c)" and base_vars = term.vars
-proof unfold_locales
-  fix c and \<rho> :: "('f, 'v) subst"
-  assume "context.is_renaming \<rho>" 
-  then have "\<And>t. Var ` term.vars (c\<langle>t\<rangle> \<cdot>t \<rho>) = \<rho> ` term.vars c\<langle>t\<rangle>"
-    by (meson term.renaming_variables)
-  
-  then show "Var ` context.vars (c \<cdot>t\<^sub>c \<rho>) = \<rho> ` context.vars c"
-    unfolding vars_term_ctxt_apply subst_apply_term_ctxt_apply_distrib
-    by (metis Un_commute Un_empty_left is_ground_trm_iff_ident_forall_subst term.ground_exists)
-next
-  fix c unifiers and \<mu> :: "('f, 'v) subst"
-  assume "finite unifiers" "\<forall>U\<in>unifiers. finite U" "term_subst.is_imgu \<mu> unifiers"
-  
-  then have "\<And>t. term.vars (c\<langle>t\<rangle> \<cdot>t \<mu>) \<subseteq> term.vars c\<langle>t\<rangle> \<union> \<Union> (term.vars ` \<Union> unifiers)"
-    using term.vars_imgu
-    by meson
-
-  then show "context.vars (c \<cdot>t\<^sub>c \<mu>) \<subseteq> context.vars c \<union> \<Union> (term.vars ` \<Union> unifiers)"
-    unfolding vars_term_ctxt_apply subst_apply_term_ctxt_apply_distrib
-    by (metis le_sup_iff sup_bot.right_neutral term.ground_exists)
-qed*)
 
 lemma ground_ctxt_iff_context_is_ground: "ground_ctxt c \<longleftrightarrow> context.is_ground c"
   by(induction c)(simp_all add: term_context_ground_iff_term_is_ground)
+
+lemma ground_term_with_context1:
+  assumes "context.is_ground c" "term.is_ground t"
+  shows "(context.to_ground c)\<langle>term.to_ground t\<rangle>\<^sub>G = term.to_ground c\<langle>t\<rangle>"
+  using assms
+  unfolding context.to_ground_def
+  by(induction c) simp_all
+
+lemma ground_term_with_context2:
+  assumes "context.is_ground c"  
+  shows "term.from_ground (context.to_ground c)\<langle>t\<^sub>G\<rangle>\<^sub>G = c\<langle>term.from_ground t\<^sub>G\<rangle>"
+  using assms
+  unfolding context.to_ground_def
+  by(induction c) (simp_all add: context.to_ground_def map_idI)
+
+lemma ground_term_with_context3: 
+  "(context.from_ground c\<^sub>G)\<langle>term.from_ground t\<^sub>G\<rangle> = term.from_ground c\<^sub>G\<langle>t\<^sub>G\<rangle>\<^sub>G"
+  using ground_term_with_context2[OF context.ground_is_ground, symmetric]
+  unfolding context.from_ground_inverse.
+
+lemmas ground_term_with_context =
+  ground_term_with_context1
+  ground_term_with_context2
+  ground_term_with_context3
+
+lemma context_is_ground_context_compose1:
+  assumes "context.is_ground (c \<circ>\<^sub>c c')"
+  shows "context.is_ground c" "context.is_ground c'"
+  using assms
+  by(induction c) auto
+
+lemma context_is_ground_context_compose2:
+  assumes "context.is_ground c" "context.is_ground c'" 
+  shows "context.is_ground (c \<circ>\<^sub>c c')"
+  using assms
+  by (meson ground_ctxt_comp ground_ctxt_iff_context_is_ground)
+
+lemmas context_is_ground_context_compose = 
+  context_is_ground_context_compose1 
+  context_is_ground_context_compose2
+
+lemma ground_context_subst:
+  assumes 
+    "context.is_ground c\<^sub>G" 
+    "c\<^sub>G = (c \<cdot>t\<^sub>c \<sigma>) \<circ>\<^sub>c c'"
+  shows 
+    "c\<^sub>G = c \<circ>\<^sub>c c' \<cdot>t\<^sub>c \<sigma>"
+  using assms 
+proof(induction c)
+  case Hole
+  then show ?case
+    by simp
+next
+  case More
+  then show ?case
+    using context_is_ground_context_compose1(2)
+    by (metis subst_compose_ctxt_compose_distrib context.subst_ident_if_ground)
+qed
+
+lemma context_from_ground_hole: "context.from_ground c\<^sub>G = \<box> \<longleftrightarrow> c\<^sub>G = \<box>"
+  by(cases c\<^sub>G) (simp_all add: context.from_ground_def)
+
+lemma term_with_context_is_ground: "term.is_ground c\<langle>t\<rangle> \<longleftrightarrow> context.is_ground c \<and> term.is_ground t"
+  by simp
 
 end
