Superposition_Calculus/Term_Rewrite_System.thy
@@ -1,7 +1,7 @@
 theory Term_Rewrite_System
   imports
     Isabelle_2024_Compatibility
-    Ground_Ctxt_Extra
+    Ground_Context
 begin
 
 definition compatible_with_gctxt :: "'f gterm rel \<Rightarrow> bool" where
